src/Examples.v
@@ -1,0 +1,78 @@
+(* Celsius project *)
+(* Clément Blaudeau - Lamp@EPFL & Inria 2020-2022 *)
+(* ------------------------------------------------------------------------ *)
+(* This files shows the examples of the paper. To check it, replace the definition of the parameters
+in Language.v with those, and rerun the proofs up to the soundness theorem. I plan to make it
+cleaner with a centralized import. *)
+
+
+(* ------------------------------------------------------------------------ *)
+(** ** Example 1 *)
+(*
+
+class A () {
+ var b = new B(this)
+}
+
+class B (x : (A,cold)) {
+ var a = x
+}
+
+class Entry () {
+ def main() {
+   new A()
+ }
+}
+
+*)
+
+(** ** Definitions *)
+(* To put in Language.v *)
+
+Definition A := cln(1).
+Definition B := cln(2).
+Definition Entry := cln(0).
+Definition EntryClass :=
+  class nil nil (fun m => if (let 'mtd n := m in PeanoNat.Nat.eqb n 0)
+                       then Some (method hot nil (A,hot) (e_new A nil))
+                       else None).
+
+Definition Ξ : list Class :=
+  [(* Main Class *)
+    EntryClass;
+
+    (* Class A *)
+    class nil [field (B,warm) (e_new B [e_this])] (fun _ => None);
+
+    (* Class B *)
+    class [(A,cold)] [field (A,cold) (e_var 0)] (fun _ => None)
+  ].
+
+Lemma EntryClass_ct : ct Entry = EntryClass.
+Proof. unfold ct, Entry. simpl. reflexivity. Qed.
+
+(** ** Typing *)
+(* To put in Soundness.v *)
+
+Lemma typable_classes : T_Classes.
+Proof with (unfold A, B, Entry; simpl; eauto with typ).
+  unfold T_Classes.
+  intros [c].
+  assert (c = 1 \/ c = 2 \/ (c = 0 \/ c > 2)) as [|[|]] by lia; subst; simpl.
+  - (* Class A *)
+    split.
+    + eapply t_fields_cool_cons; eauto using T_Fields.
+      eapply t_new...
+    + intros. inverts H.
+  - (* Class B *)
+    split.
+    + eapply t_fields_cool_cons ; eauto using T_Fields.
+      eapply t_var...
+    + intros. inverts H.
+  - (* Class Entry *)
+    assert (P_hots []) by (unfold P_hots; eauto using Forall).
+    steps; try lia...
+    + eapply t_new_hot...
+    + eapply t_new_hot...
+    + eapply t_new_hot...
+Qed.
